Finish proving/using that SymexLines scribles only over known memory
What remains is doing the reverse of the final symex goal to deal with
the different representations of memory specs, splitting apart input and
output values via `++` (not 100% sure how to do this yet), and showing
that the outputs are mapped to the right values (also need to figure out
how to do this).

src/Assembly/WithBedrock/Proofs.v
@@ -26,6 +26,7 @@ Require Import Crypto.Util.ListUtil.
 Require Import Crypto.Util.ListUtil.FoldMap.
 Require Import Crypto.Util.ListUtil.Forall.
 Require Import Crypto.Util.ListUtil.IndexOf.
+Require Import Crypto.Util.ListUtil.Split.
 Require Import Crypto.Util.OptionList.
 Require Import Crypto.Util.ZUtil.Definitions.
 Require Import Crypto.Util.ZUtil.AddGetCarry.
@@ -42,6 +43,7 @@ Require Import Crypto.Util.ZUtil.Tactics.PeelLe.
 Require Import Crypto.Util.Tactics.BreakMatch.
 Require Import Crypto.Util.Tactics.SpecializeBy.
 Require Import Crypto.Util.Tactics.HasBody.
+Require Import Crypto.Util.Tactics.Head.
 Require Import Crypto.Util.Tactics.PrintContext.
 Require Import Crypto.Util.Tactics.PrintGoal.
 Require Import Crypto.Util.Tactics.UniquePose.
@@ -3536,6 +3538,311 @@ Proof.
   reflexivity.
 Qed.
 
+Definition same_mem_addressed (s1 s2 : mem_state) : Prop
+  := List.map fst s1 = List.map fst s2.
+
+Lemma update_nth_fst_mem_same m1 n y
+  : same_mem_addressed m1 (update_nth n (fun ptsto : idx * idx => (fst ptsto, y)) m1).
+Proof.
+  revert n m1.
+  cbv [same_mem_addressed]; induction n as [|n IH], m1 as [|? m1]; cbn [update_nth List.map fst]; f_equal; eauto.
+Qed.
+
+(* TODO: move? *)
+Lemma store_mem_same x y m1 m2 (H : store x y m1 = Some m2)
+  : same_mem_addressed m1 m2.
+Proof.
+  cbv [store Crypto.Util.Option.bind] in *; break_innermost_match_hyps; inversion_option; subst.
+  apply update_nth_fst_mem_same.
+Qed.
+
+Class same_mem_addressed_of_success {T} (f : M T)
+  := success_same_mem : forall v s s', f s = Success (v, s') -> same_mem_addressed s s'.
+
+Local Ltac same_mem_addressed_of_success_t_step_normal_nobreak :=
+  first [ progress cbv [same_mem_addressed_of_success] in *
+        | progress intros
+        | reflexivity
+        | assumption
+        | progress inversion_ErrorT
+        | progress destruct_head'_prod
+        | progress cbn [fst snd Symbolic.symbolic_mem_state] in *
+        | progress cbv [update_dag_with update_mem_with update_flag_with update_reg_with Symbolic.bind Symbolic.ret Symbolic.err some_or ErrorT.bind] in *
+        | progress inversion_pair
+        | progress subst
+        | match goal with
+          | [ H : store _ _ _ = Some _ |- _ ] => apply store_mem_same in H
+          | [ H : _ = Success _ |- _ ] => apply success_same_mem in H
+          end
+        | cbv [same_mem_addressed] in *; congruence ].
+
+Local Ltac same_mem_addressed_of_success_t_step_normal :=
+  first [ same_mem_addressed_of_success_t_step_normal_nobreak
+        | break_innermost_match_hyps_step ].
+
+Local Ltac same_mem_addressed_of_success_t_step_unfold :=
+  match goal with
+  | [ H : ?f = Success _ |- _ ]
+    => let f' := head f in
+       idtac f';
+       progress unfold f' in H
+  end.
+
+Local Ltac same_mem_addressed_of_success_t_step_unfold_go :=
+  repeat same_mem_addressed_of_success_t_step_normal;
+  same_mem_addressed_of_success_t_step_unfold;
+  repeat same_mem_addressed_of_success_t_step_normal.
+
+Local Ltac same_mem_addressed_of_success_t := repeat first [ same_mem_addressed_of_success_t_step_normal | same_mem_addressed_of_success_t_step_unfold ].
+
+(* TODO: move? *)
+Local Instance Merge_mem_same x : same_mem_addressed_of_success (Symbolic.Merge x).
+Proof. same_mem_addressed_of_success_t. Qed.
+
+(* TODO: move? *)
+Local Instance App_mem_same x : same_mem_addressed_of_success (Symbolic.App x).
+Proof. same_mem_addressed_of_success_t. Qed.
+
+(* TODO: move? *)
+Local Instance GetReg_mem_same r : same_mem_addressed_of_success (GetReg r).
+Proof. same_mem_addressed_of_success_t. Qed.
+
+(* TODO: move? *)
+Local Instance Address_mem_same sa a : same_mem_addressed_of_success (@Address sa a).
+Proof. same_mem_addressed_of_success_t. Qed.
+
+(* TODO: move? *)
+Local Instance GetOperand_mem_same sz sa arg : same_mem_addressed_of_success (@GetOperand sz sa arg).
+Proof. same_mem_addressed_of_success_t. Qed.
+
+(* TODO: move? *)
+Local Instance GetFlag_mem_same f : same_mem_addressed_of_success (GetFlag f).
+Proof. same_mem_addressed_of_success_t. Qed.
+
+(* TODO: move? *)
+Local Instance SetOperand_mem_same sz sa arg v : same_mem_addressed_of_success (@SetOperand sz sa arg v).
+Proof. same_mem_addressed_of_success_t. Qed.
+
+(* TODO: move? *)
+Local Instance SetFlag_mem_same f v : same_mem_addressed_of_success (SetFlag f v).
+Proof. same_mem_addressed_of_success_t. Qed.
+
+(* TODO: move? *)
+Local Instance RevealConst_mem_same v : same_mem_addressed_of_success (RevealConst v).
+Proof. same_mem_addressed_of_success_t. Qed.
+
+(* TODO: move? *)
+Local Instance Reveal_mem_same v1 v2 : same_mem_addressed_of_success (Reveal v1 v2).
+Proof. same_mem_addressed_of_success_t. Qed.
+
+(* TODO: move? *)
+Local Instance HavocFlags_mem_same : same_mem_addressed_of_success HavocFlags.
+Proof. same_mem_addressed_of_success_t. Qed.
+
+(* TODO: move? *)
+Local Instance ret_mem_same {T} (v : T) : same_mem_addressed_of_success (ret v).
+Proof. same_mem_addressed_of_success_t. Qed.
+
+(* TODO: move? *)
+Local Instance bind_mem_same {A B} f v
+      {H0 : same_mem_addressed_of_success v}
+      {H1 : forall v', same_mem_addressed_of_success (f v')}
+  : same_mem_addressed_of_success (@Symbolic.bind A B v f).
+Proof.
+  same_mem_addressed_of_success_t.
+  specialize (H0 _ _ _ ltac:(eassumption)).
+  specialize (H1 _ _ _ _ ltac:(eassumption)).
+  cbv [same_mem_addressed] in *; congruence.
+Qed.
+
+(* TODO: move? *)
+Local Instance mapM_mem_same {A B} f ls
+      {H1 : forall v', same_mem_addressed_of_success (f v')}
+  : same_mem_addressed_of_success (@mapM A B f ls).
+Proof.
+  induction ls as [|?? IH]; cbn [mapM];
+    same_mem_addressed_of_success_t.
+  specialize (IH _ _ _ ltac:(eassumption)).
+  specialize (H1 _ _ _ _ ltac:(eassumption)).
+  same_mem_addressed_of_success_t.
+Defined.
+
+(* TODO: move? *)
+Fixpoint Symeval_mem_same sz sa args {struct args} : same_mem_addressed_of_success (@Symeval sz sa args).
+Proof.
+  destruct args; cbn [Symeval] in *; typeclasses eauto.
+Qed.
+Local Existing Instance Symeval_mem_same.
+Typeclasses Opaque Symeval.
+Typeclasses Transparent AddressSize OperationSize.
+
+(* TODO: move? *)
+Local Instance SymexNormalInstruction_mem_same instr : same_mem_addressed_of_success (SymexNormalInstruction instr).
+Proof.
+  destruct instr; cbv [SymexNormalInstruction err Symbolic.bind ret Syntax.op Syntax.args ErrorT.bind same_mem_addressed_of_success] in *; intros.
+  same_mem_addressed_of_success_t.
+Qed.
+
+(* TODO: move? *)
+Local Instance SymexLine_mem_same line : same_mem_addressed_of_success (SymexLine line).
+Proof.
+  cbv [SymexLine SymexRawLine err ret] in *; break_innermost_match; try congruence.
+  typeclasses eauto.
+Qed.
+
+(* TODO: move? *)
+Lemma SymexLines_mem_same lines s s'
+      (H : SymexLines lines s = Success (tt, s'))
+  : same_mem_addressed s s'.
+Proof.
+  revert s H.
+  induction lines as [|line lines IH]; cbn [SymexLines]; cbv [Symbolic.ret Symbolic.bind ErrorT.bind]; intros *; break_innermost_match; intros; inversion_ErrorT; inversion_pair; subst; try reflexivity.
+  specialize (IH _ ltac:(eassumption)).
+  same_mem_addressed_of_success_t.
+Qed.
+
+Lemma same_mem_addressed_alt l1 l2
+      (H : same_mem_addressed l1 l2)
+  : exists l2b, List.combine (List.map fst l1) l2b = l2 /\ List.length l2b = List.length l1.
+Proof.
+  cbv [same_mem_addressed] in *.
+  rewrite H.
+  pose proof (split_combine l2) as H'.
+  rewrite split_alt in H'.
+  eexists; split; [ eassumption | ].
+  apply (f_equal (@List.length _)) in H.
+  rewrite !map_length in *; congruence.
+Qed.
+
+Lemma same_mem_addressed_app_ex_r l1 l2 l3
+      (H : same_mem_addressed (l1 ++ l2) l3)
+  : exists l3a l3b, l3a ++ l3b = l3 /\ same_mem_addressed l1 l3a /\ same_mem_addressed l2 l3b.
+Proof.
+  cbv [same_mem_addressed] in *.
+  rewrite map_app in H.
+  exists (firstn (List.length l1) l3), (skipn (List.length l1) l3).
+  rewrite <- firstn_map, <- skipn_map, <- H, firstn_app, skipn_app, map_length, Nat.sub_diag, firstn_O, skipn_O, firstn_skipn, firstn_all, (skipn_all (List.length l1)), app_nil_l, app_nil_r by now rewrite map_length; lia.
+  auto.
+Qed.
+
+Lemma same_mem_addressed_rev_ex_r l1 l2
+      (H : same_mem_addressed (List.rev l1) l2)
+  : exists l3, List.rev l3 = l2 /\ same_mem_addressed l1 l3.
+Proof.
+  cbv [same_mem_addressed] in *.
+  exists (List.rev l2).
+  rewrite map_rev, <- H, map_rev, !rev_involutive.
+  auto.
+Qed.
+
+Lemma same_mem_addressed_combine_ex_r_helper l1a l1b l2
+      (H : same_mem_addressed (List.combine l1a l1b) l2)
+  : exists l2b, List.combine (firstn (List.length l1b) l1a) l2b = l2.
+Proof.
+  cbv [same_mem_addressed] in *.
+  exists (List.map snd l2).
+  rewrite map_fst_combine in H.
+  pose proof (split_combine l2) as H'.
+  rewrite split_alt, <- H in H'.
+  assumption.
+Qed.
+
+Lemma same_mem_addressed_combine_ex_r l1a l1b l2
+      (H : same_mem_addressed (List.combine l1a l1b) l2)
+  : exists l2b, List.combine l1a l2b = l2.
+Proof.
+  apply same_mem_addressed_combine_ex_r_helper in H.
+  destruct H as [l2b H].
+  exists (firstn (List.length l1b) l2b).
+  subst.
+  etransitivity; rewrite combine_truncate_l, combine_truncate_r; [ | reflexivity ].
+  rewrite ?firstn_length, ?firstn_firstn_min.
+  do 2 f_equal; lia.
+Qed.
+
+Lemma same_mem_addressed_nil ls
+      (H : same_mem_addressed nil ls)
+  : nil = ls.
+Proof.
+  destruct ls; cbv in H; congruence.
+Qed.
+
+Lemma same_mem_addressed_init_symbolic_state d ls
+      (H : same_mem_addressed (init_symbolic_state d) ls)
+  : symbolic_mem_state (init_symbolic_state d) = ls.
+Proof.
+  cbv [init_symbolic_state] in *.
+  break_innermost_match_hyps.
+  apply same_mem_addressed_nil, H.
+Qed.
+
+Lemma same_mem_addressed_flat_map_combine_addrs_ex_r {dereference_scalar:bool} {T} (ls1 : list (_ + T * _)) ls2 ls'
+      (H : same_mem_addressed (List.flat_map
+                                 (fun '(idx', idx)
+                                  => match idx', idx with
+                                     | inl addr_or_val, inl val => if dereference_scalar then [(addr_or_val, val)] else []
+                                     | inl _, _ | _, inl _ => []
+                                     | inr (base', addrs'), inr items
+                                       => List.combine addrs' items
+                                     end)
+                                 (List.combine ls1 ls2))
+                              ls')
+  : exists ls'2, List.flat_map
+                   (fun '(idx', idx)
+                    => match idx', idx with
+                       | inl addr_or_val, inl val => if dereference_scalar then [(addr_or_val, val)] else []
+                       | inl _, _ | _, inl _ => []
+                       | inr (base', addrs'), inr items
+                         => List.combine addrs' items
+                       end)
+                   (List.combine ls1 ls'2) = ls'.
+Proof.
+  revert dependent ls'.
+  revert ls1 ls2.
+  induction ls1 as [|?? IH], ls2 as [|? ls2];
+    try specialize (IH ls2);
+    cbn [List.combine List.map List.flat_map]; intros.
+  all: repeat first [ progress subst
+                    | progress destruct_head'_and
+                    | progress destruct_head'_ex
+                    | (now exists nil)
+                    | specialize (IH _ ltac:(eassumption))
+                    | match goal with
+                      | [ H : same_mem_addressed nil _ |- _ ] => apply same_mem_addressed_nil in H
+                      | [ H : same_mem_addressed (_ ++ _) _ |- _ ] => apply same_mem_addressed_app_ex_r in H
+                      | [ H : nil = List.map _ ?ls |- _ ] => is_var ls; destruct ls
+                      | [ H : same_mem_addressed match _ with _ => _ end ?x |- _ ]
+                        => is_var x; apply same_mem_addressed_alt in H
+                      end ].
+  eexists (_ :: _); cbn [flat_map]; apply f_equal2; [ | reflexivity ].
+  repeat first [ match goal with
+                 | [ |- match ?x with _ => _ end = List.combine (List.map _ match ?x with _ => _ end) _ ]
+                   => destruct x
+                 | [ |- match ?ev with inl _ => _ | inr _ => nil end = List.combine (List.map _ match ?x with inl _ => _ | inr _ => nil end) _ ]
+                   => is_evar ev;
+                      is_var x;
+                      let __ := open_constr:(eq_refl : ev = match x with inl _ => inl _ | inr _ => inr _ end) in
+                      destruct x
+                 | [ |- [(_, ?ev)] = match ?x with _ => _ end ]
+                   => is_evar ev;
+                      is_var x;
+                      let __ := open_constr:(eq_refl : ev = match x with nil => _ | _ :: _ => _ end) in
+                      destruct x
+                 | [ |- List.combine ?ls ?ev = List.combine (firstn (List.length ?ls') ?ls) ?x ]
+                   => is_evar ev; unify ev (firstn (List.length ls') x)
+                 end
+               | exfalso; discriminate
+               | reflexivity
+               | rewrite map_fst_combine
+               | progress cbn [List.map List.combine fst List.length] in *
+               | break_innermost_match_step ].
+  etransitivity; rewrite combine_truncate_l, combine_truncate_r; [ | reflexivity ].
+  rewrite ?firstn_length, ?firstn_firstn_min.
+  do 2 f_equal; lia.
+  Unshelve.
+  all: assumption.
+Qed.
+
 Import Coq.Strings.String.
 Import Coq.Lists.List.
 Import Crypto.Util.Option.
@@ -3706,6 +4013,24 @@ Local Ltac handle_R_regs _ :=
       debug_run ltac:(fun _ => idtac "R => R_regs set_reg end")
   end.
 
+Local Ltac handle_same_mem :=
+  repeat first [ progress subst
+               | progress destruct_head'_ex
+               | progress destruct_head'_and
+               | match goal with
+                 | [ H : same_mem_addressed nil _ |- _ ] => apply same_mem_addressed_nil in H
+                 | [ H : same_mem_addressed (_ ++ _)%list _ |- _ ] => apply same_mem_addressed_app_ex_r in H
+                 | [ H : same_mem_addressed (List.rev _) _ |- _ ] => apply same_mem_addressed_rev_ex_r in H
+                 | [ H : same_mem_addressed (List.flat_map _ _) _ |- _ ]
+                   => apply (same_mem_addressed_flat_map_combine_addrs_ex_r (dereference_scalar:=false)) in H
+                 | [ H : same_mem_addressed (List.flat_map _ _) _ |- _ ]
+                   => apply (same_mem_addressed_flat_map_combine_addrs_ex_r (dereference_scalar:=true)) in H
+                 | [ H : same_mem_addressed (symbolic_mem_state (init_symbolic_state _)) _ |- _ ]
+                   => apply same_mem_addressed_init_symbolic_state in H
+                 | [ H : same_mem_addressed (List.combine _ _) _ |- _ ]
+                   => apply same_mem_addressed_combine_ex_r in H
+                 end ].
+
 Theorem symex_asm_func_M_correct
         d frame asm_args_out asm_args_in (G : symbol -> option Z) (s := init_symbolic_state d)
         (s' : symbolic_state) (m : machine_state) (output_types : type_spec) (stack_size : nat) (stack_base : Naive.word 64)
@@ -3867,6 +4192,8 @@ Proof.
                       debug_run ltac:(fun _ => idtac "get callee_saved_registers end")
                  | [ H : SymexLines _ _ = Success _ |- exists m' : machine_state, _ ]
                    => debug_run ltac:(fun _ => idtac "SymexLines start");
+                      let H' := fresh in
+                      pose proof H as H'; apply SymexLines_mem_same in H';
                       eapply SymexLines_R in H;
                       [ destruct H as [m' H];
                         exists m', G_final;
@@ -3942,7 +4269,7 @@ Proof.
                       debug_run ltac:(fun _ => idtac "Forall2_rets_of_R_mem end")
                  end
                | progress repeat (apply conj; eauto 10; []) ].
-  all: destruct_head' symbolic_state; cbn [update_dag_with Symbolic.dag_state Symbolic.symbolic_flag_state Symbolic.symbolic_mem_state Symbolic.symbolic_reg_state] in *; subst.
+  all: destruct_head' symbolic_state; cbn [update_dag_with Symbolic.dag_state Symbolic.symbolic_flag_state Symbolic.symbolic_mem_state Symbolic.symbolic_reg_state] in *; subst; handle_same_mem.
   { cbv [R_runtime_output R update_dag_with] in *; destruct_head'_and.
     do 2 eexists.
     repeat match goal with |- _ /\ _ => split end.
